Move refl/sym/trans of Sequiv to EquivFacts
Having these theorems in separate files just made the codebase more
confusing.

On the way, we delete a lot of unnecessary stuff in Rel.

src/EquivFacts.v
@@ -1,43 +1,198 @@
 Require Import Contractive ContractiveFacts CS CSFacts Equiv Free FreeFacts
-  NonEquiv Sty StyInd Subst SubstFacts Shape Symmetry Tac Msg Var Wf.
+  NonEquiv Rel Sty StyInd Subst SubstFacts Shape Tac Msg Var Wf WfFacts.
 Require Import TLC.LibRelation TLC.LibLogic.
 
-(* --------------------------------------------------------------------------*)
-(* Automation *)
 
-Lemma Sequiv_var_absurd_l :
-  forall S X,
-  Contractive S ->
-  ~ Sequiv (var X) S.
+(* ------------------------------------------------------------------------- *)
+(* Reflexivity *)
+
+Inductive R_Sequiv_reflexive : Sty -> Sty -> Prop :=
+| R_Sequiv_reflexive_refl :
+    forall S,
+    Wf S ->
+    R_Sequiv_reflexive S S
+| R_Sequiv_reflexive_mu1 :
+    forall X S,
+    Wf (subst X (mu X S) S) ->
+    R_Sequiv_reflexive (mu X S) (subst X (mu X S) S)
+| R_Sequiv_reflexive_mu2 :
+    forall X S,
+    Wf (subst X (mu X S) S) ->
+    R_Sequiv_reflexive (subst X (mu X S) S) (mu X S)
+.
+
+Theorem Sequiv_reflexive :
+  forall S,
+  Wf S ->
+  Sequiv S S.
 Proof.
-  induction S using (well_founded_ind lt_Sty_mu_prefix_wf);
-    introv Hcontr contra; inverts2 contra.
-  - eapply H with (y := subst X0 (mu X0 S') S'); eauto with contractive subst.
+  intros. apply Sequiv_coind with (R := R_Sequiv_reflexive);
+    [|constructor; auto].
+  clear. introv H. inverts1 H; [destruct S'|..];
+    try (constructor; constructor); auto with wf.
 Qed.
 
-Hint Extern 4 =>
-  match goal with
-  | H : Sequiv (var ?X) ?S |- _ =>
-      exfalso; apply (Sequiv_var_absurd_l S X); [|assumption]
-  end
+
+(* ------------------------------------------------------------------------- *)
+(* Symmetry *)
+
+
+Theorem Sequiv_symmetric : forall S S',
+  Sequiv S S' -> Sequiv S' S.
+Proof with auto.
+  apply clos_sym_sym. unfold inclusion. apply Sequiv_coind.
+  intros S S' H.
+  inversion_clear H. inversion_clear H0.
+  inversion H; constructor; subst; constructor...
+Qed.
+
+
+(* ------------------------------------------------------------------------- *)
+(* Transitivity *)
+
+
+Create HintDb sequiv_trans discriminated.
+Hint Resolve Sequiv_reflexive : sequiv_trans.
+
+
+Inductive R_Sequiv_transitive : Sty -> Sty -> Prop :=
+| R_Sequiv_transitive_intro :
+    forall S T U,
+    Wf S ->
+    Wf T ->
+    Wf U ->
+    Sequiv S T ->
+    Sequiv T U ->
+    R_Sequiv_transitive S U
 .
+Hint Constructors R_Sequiv_transitive : sequiv_trans.
+
+Lemma R_Sequiv_transitive_reflexive :
+  forall S,
+  Wf S ->
+  R_Sequiv_transitive S S.
+Proof. eauto with sequiv_trans. Qed.
+
+Lemma Sequiv_R_Sequiv_transitive :
+  forall S T,
+  Wf S ->
+  Wf T ->
+  Sequiv S T ->
+  R_Sequiv_transitive S T.
+Proof. eauto with sequiv_trans. Qed.
 
 
-Lemma Sequiv_var_absurd_r :
-  forall S X,
-  Contractive S ->
-  ~ Sequiv S (var X).
-Proof. introv Hok contra. apply Sequiv_symmetric in contra. auto. Qed.
+(* TODO beautify (a lot) *)
+Theorem Sequiv_transitive :
+  forall S T U,
+  Wf S ->
+  Wf T ->
+  Wf U ->
+  Sequiv S T ->
+  Sequiv T U ->
+  Sequiv S U.
+Proof.
+  intros. apply Sequiv_coind with (R := R_Sequiv_transitive);
+    [|eauto with sequiv_trans].
+  clear. introv H. rename S' into U. inverts H.
+  assert (Sequiv S (cs T)) as HSeqT  by (
+    eapply cs_preserves_Sequiv_r; eauto with wf
+  ).
+  assert (Sequiv (cs T) U) as HTeqU by (
+    eapply cs_preserves_Sequiv_l; eauto with wf
+  ).
+  clear H3 H4. inverts2 HSeqT; inverts2 HTeqU; subst; try solve [false].
 
-Hint Extern 4 =>
-  match goal with
-  | H : Sequiv ?S (var ?X) |- _ =>
-      exfalso; apply (Sequiv_var_absurd_r S X); [|assumption]
-  end
-.
+  (* unit *)
+  - auto.
+
+  - constructor. rewrite <- HSeqT in *.
+    apply Sequiv_R_Sequiv_transitive; auto with wf.
+
+  (* send *)
+  - rewrite <- H4 in H3. injection H3; intros; subst.
+    constructor. apply R_Sequiv_transitive_intro with (T := S); eauto with wf.
+      apply cs_preserves_Wf in H1. rewrite <- H4 in H1.
+      eauto with wf.
+
+  - constructor. rewrite <- H3 in *.
+    apply R_Sequiv_transitive_intro with (T := send B S'); eauto with wf.
+      rewrite H3. eauto with wf.
+
+  (* recv *)
+  - rewrite <- H4 in H3. injection H3; intros; subst.
+    constructor. apply R_Sequiv_transitive_intro with (T := S); eauto with wf.
+      apply cs_preserves_Wf in H1. rewrite <- H4 in H1.
+      eauto with wf.
+
+  - constructor. rewrite <- H3 in *.
+    apply R_Sequiv_transitive_intro with (T := recv B S'); eauto with wf.
+      rewrite H3. eauto with wf.
+
+  (* echoice *)
+  - assert (Wf (echoice S1' S2')) by (rewrite H3; eauto with wf).
+    rewrite <- H4 in H3. injection H3; intros; subst.
+    constructor.
+    * apply R_Sequiv_transitive_intro with (T := S0); eauto with wf.
+    * apply R_Sequiv_transitive_intro with (T := S3); eauto with wf.
+
+  - assert (Wf (echoice S1' S2')) by (rewrite H3; eauto with wf).
+    constructor. rewrite <- H3 in *.
+    apply R_Sequiv_transitive_intro with (T := echoice S1' S2'); eauto with wf.
+
+  (* ichoice *)
+  - assert (Wf (ichoice S1' S2')) by (rewrite H3; eauto with wf).
+    rewrite <- H4 in H3. injection H3; intros; subst.
+    constructor.
+    * apply R_Sequiv_transitive_intro with (T := S0); eauto with wf.
+    * apply R_Sequiv_transitive_intro with (T := S3); eauto with wf.
+
+  - assert (Wf (ichoice S1' S2')) by (rewrite H3; eauto with wf).
+    constructor. rewrite <- H3 in *.
+    apply R_Sequiv_transitive_intro with (T := ichoice S1' S2'); eauto with wf.
+
+  (* unit *)
+  - rewrite <- HTeqU in *. constructor. apply Sequiv_R_Sequiv_transitive;
+      auto with wf.
+
+  (* send *)
+  - constructor. rewrite <- H3 in *.
+    apply R_Sequiv_transitive_intro with (T := send B S); auto with wf.
+      rewrite H3; eauto with wf.
+
+  (* recv *)
+  - constructor. rewrite <- H3 in *.
+    apply R_Sequiv_transitive_intro with (T := recv B S); auto with wf.
+      rewrite H3; eauto with wf.
+
+  (* echoice *)
+  - constructor. rewrite <- H3 in *.
+    apply R_Sequiv_transitive_intro with (T := echoice S1 S2); auto with wf.
+      rewrite H3; eauto with wf.
+
+  (* ichoice *)
+  - constructor. rewrite <- H3 in *.
+    apply R_Sequiv_transitive_intro with (T := ichoice S1 S2); auto with wf.
+      rewrite H3; eauto with wf.
+
+  (* mu 1 (impossible) *)
+  - exfalso; eauto with subst wf.
+
+  (* mu 2 *)
+  - constructor.
+    assert (Sequiv (cs T) (mu X0 S')) as HTeqU' by auto.
+    apply R_Sequiv_transitive_intro with (T := cs T);
+      eauto with wf.
+
+  (* mu 3 (impossible) *)
+  - exfalso; eauto with subst wf.
+
+  (* mu 4 (impossible) *)
+  - exfalso; eauto with subst wf.
+Qed.
 
 
-(* --------------------------------------------------------------------------*)
+(* ------------------------------------------------------------------------- *)
 (* NSequiv -> ~ Sequiv *)
 
 
@@ -62,7 +217,7 @@ Proof.
 Qed.
 
 
-(* --------------------------------------------------------------------------*)
+(* ------------------------------------------------------------------------- *)
 (* ~ NSequiv -> Sequiv *)
 
 
@@ -103,7 +258,7 @@ Proof.
 Qed.
 
 
-(* --------------------------------------------------------------------------*)
+(* ------------------------------------------------------------------------- *)
 (* NSequiv <-> ~ Sequiv *)
 
 Lemma NSequiv_iff_not_Sequiv :
