src/Rel.v
@@ -1,11 +1,11 @@
 Require Import Tac.
 Require Export Relations.
-Require TLC.LibRelation.
+
 
 Create HintDb rel discriminated.
 Hint Unfold inclusion : rel.
 Hint Unfold symmetric : rel.
-Hint Unfold transitive : rel.
+
 
 Inductive clos_sym A (R : relation A) : relation A :=
 | clos_sym_intro : forall x y : A, R x y -> clos_sym A R y x
@@ -13,60 +13,9 @@ Inductive clos_sym A (R : relation A) : relation A :=
 Hint Constructors clos_sym : rel.
 Hint Constructors clos_trans : rel.
 
+
 Lemma clos_sym_sym :
   forall A (R : relation A),
   inclusion A (clos_sym A R) R ->
   symmetric A R.
 Proof. auto with rel. Qed.
-
-Lemma clos_trans_trans :
-  forall A (R : relation A),
-  inclusion A (clos_trans A R) R ->
-  transitive A R.
-Proof.
-  unfold inclusion. unfold transitive. eauto with rel.
-Qed.
-
-Inductive clos_trans' {A} (R : relation A) : relation A :=
-| clos_trans'_intro :
-    forall x y z,
-    R x y -> R y z -> clos_trans' R x z
-.
-Hint Constructors clos_trans' : rel.
-
-Lemma clos_trans'_trans :
-  forall A R,
-  inclusion A (clos_trans' R) R ->
-  transitive A R.
-Proof. eauto with rel. Qed.
-
-(* -------------------------------------------------------------------------- *)
-(* Conversion between LibRelation and Coq standard library *)
-
-Ltac solve_LibRelation_conversion :=
-  let H := fresh in
-  intros; split; introv H; red in H; red; eauto.
-
-Lemma reflexive_refl_iff {A} {R} :
-  reflexive A R <-> TLC.LibRelation.refl R.
-Proof. solve_LibRelation_conversion. Qed.
-
-Lemma refl_reflexive {A} {R} :
-  TLC.LibRelation.refl R -> reflexive A R.
-Proof. intros; apply reflexive_refl_iff; auto. Qed.
-
-Lemma symmetric_sym_iff {A} {R} :
-  symmetric A R <-> TLC.LibRelation.sym R.
-Proof. solve_LibRelation_conversion. Qed.
-
-Lemma sym_symmetric {A} {R} :
-  TLC.LibRelation.sym R -> symmetric A R.
-Proof. intros; apply symmetric_sym_iff; auto. Qed.
-
-Lemma transitive_trans_iff {A} {R} :
-  transitive A R <-> TLC.LibRelation.trans R.
-Proof. solve_LibRelation_conversion. Qed.
-
-Lemma trans_transitive {A} {R} :
-  TLC.LibRelation.trans R -> transitive A R.
-Proof. intros; apply transitive_trans_iff; auto. Qed.
